thys/Isabelle_Meta_Model/toy_example/embedding/core/Core_init.thy
@@ -226,7 +226,7 @@ definition "bootstrap_floor f_x l env =
 definition "wrap_toyty x = \<open>\<cdot>\<close> @@ x"
 definition "Term_annot_toy e s = Term_annot' e (wrap_toyty s)"
 definition "Term_toyset l = (case l of [] \<Rightarrow> Term_basic [\<open>Set{}\<close>] | _ \<Rightarrow> Term_paren \<open>Set{\<close> \<open>}\<close> (term_binop \<open>,\<close> l))"
-definition "Term_oid s = (\<lambda>Oid n \<Rightarrow> Term_basic [s @@ String.of_natural n])"
+definition "Term_oid s = (\<lambda>Oid n \<Rightarrow> Term_basic [s @@ String.natural_to_digit10 n])"
 
 subsection\<open>Preliminaries on: Enumeration\<close>
 
@@ -234,11 +234,11 @@ subsection\<open>Preliminaries on: Infrastructure\<close>
 
 subsection\<open>Preliminaries on: Accessor\<close>
 
-definition "print_access_oid_uniq_name' name_from_nat isub_name attr = S.flatten [ isub_name var_oid_uniq, \<open>_\<close>, String.of_natural name_from_nat, \<open>_\<close>, attr ]"
+definition "print_access_oid_uniq_name' name_from_nat isub_name attr = S.flatten [ isub_name var_oid_uniq, \<open>_\<close>, String.natural_to_digit10 name_from_nat, \<open>_\<close>, attr ]"
 definition "print_access_oid_uniq_name name_from_nat isub_name attr = print_access_oid_uniq_name' name_from_nat isub_name (String.isup attr)"
 
 definition "print_access_choose_name n i j =
-  S.flatten [var_switch, String.isub (String.of_natural n), \<open>_\<close>, String.of_natural i, String.of_natural j]"
+  S.flatten [var_switch, String.isub (String.natural_to_digit10 n), \<open>_\<close>, String.natural_to_digit10 i, String.natural_to_digit10 j]"
 
 subsection\<open>Preliminaries on: Example (Floor 1)\<close>
 
